SmallSProof.v
@@ -10,16 +10,60 @@ Require Import Coq.Relations.Operators_Properties.
 Import Assertion_S.
 Import SmallS.
 
-Definition simulation (sim : (com * continuation) -> (com * continuation) -> Prop) : Prop := forall c1 k1 c2 k2,
-  sim (c1, k1) (c2, k2) ->  (* c2 simulates c1 *)
-  (Halt c1 k1 -> (c1, k1) = (c2, k2)) /\
-  (~ Halt c1 k1 -> forall st, ~ reducible c1 k1 st -> ~ reducible c2 k2) /\
-  (* (Error c1 k1 -> Error c2 k2) /\ *)
-  (forall c1' k1' st st',
-    cstep (c1, k1, st) (c1', k1', st') ->
-    exists c2' k2',
-    mstep (c2, k2, st) (c2', k2', st') /\ sim (c1', k1') (c2', k2')).
+Lemma WP_mstep_pre: forall c k st c' k' st' Q Rb Rc,
+  WP c k Q Rb Rc st ->
+  mstep (c, k, st) (c', k', st') ->
+  WP c' k' Q Rb Rc st'.
+Proof.
+  intros.
+  remember (c, k, st) as prog.
+  remember (c', k', st') as prog'.
+  revert c k st Heqprog H.
+  unfold mstep in H0.
+  apply clos_trans_t1n_iff in H0.
+  induction H0; intros; subst.
+  - intros n.
+    specialize (H0 (S n)).
+    inversion H0; subst;
+    [ inversion H |
+      inversion H |
+      inversion H |].
+    apply (H3 _ _ _ H).
+  - destruct y as [[c'' k''] st''].
+    apply (IHclos_trans_1n eq_refl _ _ _ eq_refl).
+    intros n.
+    specialize (H1 (S n)).
+    inversion H1; subst;
+    [ inversion H |
+      inversion H |
+      inversion H |].
+    apply (H4 _ _ _ H).
+Qed.
 
+Lemma wp_sim_term : forall n c1 c2 k1 k2 Q Rb Rc st sim,
+  Halt c2 k2 \/ irreducible c2 k2 st ->
+  simulation sim ->
+  sim (c2, k2) (c1, k1) ->
+  WP_n n c1 k1 Q Rb Rc st ->
+  WP_n n c2 k2 Q Rb Rc st.
+Proof.
+  intros.
+  unfold simulation in H0.
+  pose proof halt_choice c2 k2 st as [? | [? | ?]].
+  - pose proof H0 _ _ _ _ H1 as [? _].
+    specialize (H4 H3).
+    inversion H4; subst; auto.
+  - exfalso. destruct H;
+    [ apply (halt_reducible_ex c2 k2 st); auto |
+      apply (reducible_irreducible_ex c2 k2 st); auto].
+  - pose proof H0 _ _ _ _ H1 as [_ [? _]].
+    specialize (H4 _ H3).
+    inversion H2; [constructor | | | |]; exfalso;
+    [ apply (halt_irreducible_ex c1 k1 st); auto; subst; auto_halt |
+      apply (halt_irreducible_ex c1 k1 st); auto; subst; auto_halt |
+      apply (halt_irreducible_ex c1 k1 st); auto; subst; auto_halt |]; subst.
+    apply (reducible_irreducible_ex c1 k1 st); auto.
+Qed.
 
 Lemma wp_sim : forall c1 c2 k1 k2 Q Rb Rc st sim,
   simulation sim ->
@@ -28,37 +72,112 @@ Lemma wp_sim : forall c1 c2 k1 k2 Q Rb Rc st sim,
   WP c2 k2 Q Rb Rc st.
 Proof.
   intros.
+
+  pose proof H as Hsim.
+  unfold simulation in H.
+  pose proof halt_choice c2 k2 st.
+  destruct H2 as [? | [? | ?]].
+  - pose proof H _ _ _ _ H0 as [? _].
+    specialize (H3 H2).
+    inversion H3; subst; auto.
+  - intros n.
+    revert c1 k1 c2 k2 st H0 H1 H2.
+    induction n; intros; [constructor |].
+
+    pose proof H _ _ _ _ H0 as [_ [_ ?]].
+    apply WP_Pre; auto; intros.
+    apply H3 in H4.
+    destruct H4 as (c1' & k1' & ? & ?).
+
+    pose proof WP_mstep_pre _ _ _ _ _ _ _ _ _ H1 H4.
+    pose proof halt_choice c' k' st' as [? | [? | ?]].
+    + specialize (H6 n).
+      assert (Halt c' k' \/ irreducible c' k' st'); [auto |].
+      apply (wp_sim_term _ _ _ _ _ _ _ _ _ _ H8 Hsim H5 H6).
+    + apply (IHn _ _ _ _ _ H5 H6 H7).
+    + specialize (H6 n).
+      assert (Halt c' k' \/ irreducible c' k' st'); [auto |].
+      apply (wp_sim_term _ _ _ _ _ _ _ _ _ _ H8 Hsim H5 H6).
+
+  - intros n. specialize (H1 n).
+    assert (Halt c2 k2 \/ irreducible c2 k2 st); [auto |].
+    apply (wp_sim_term _ _ _ _ _ _ _ _ _ _ H3 Hsim H0 H1).
+Qed.
+
+  (* pose proof H _ _ _ _ H0 as [_ [? _]].
+    specialize (H3 _ H2).
+    inversion H1; exfalso;
+    [ apply (halt_irreducible_ex c1 k1 st); auto; subst; auto_halt |
+      apply (halt_irreducible_ex c1 k1 st); auto; subst; auto_halt |
+      apply (halt_irreducible_ex c1 k1 st); auto; subst; auto_halt |]; subst.
+    apply (reducible_irreducible_ex c1 k1 st); auto.
+    
+
+(* ######################### *)
+
+
   revert c2 k2 H0.
   induction H1; intros.
   - unfold simulation in H.
     pose proof H1 as Hsim.
     apply H in H1.
-    pose proof halt_choice c2 k2.
+    pose proof halt_choice c2 k2 st.
     destruct H2 as [? | [? | ?]].
     + destruct H1 as [? _].
       specialize (H1 H2).
       inversion H1; subst.
       apply WP_Ter1; auto.
-    + destruct H1 as [_ [? _]].
-      specialize (H1 H2).
-      inversion H1.
-      exfalso; apply H3.
-      unfold Halt.
-      left. unfold NHalt. auto.
     + destruct H1 as [_ [_ ?]].
-      destruct H2 as (? & ? & ? & ? & ?).
+      destruct H2 as (? & ? & ? & ?).
       apply H1 in H2.
       destruct H2 as (? & ? & ? & ?).
       unfold mstep in H2.
       apply clos_trans_t1n_iff in H2.
       inversion H2; inversion H4.
+    + destruct H1 as [_ [? _]].
+      specialize (H1 _ H2).
+      inversion H1. 
   - admit.
   - admit.
   - unfold simulation in H.
+    apply H in H3.
+    pose proof halt_choice c2 k2 st.
+    destruct H4 as [? | [? | ?]].
+    + destruct H3 as [? _].
+      specialize (H3 H4).
+      inversion H3; subst.
+      exfalso; apply (halt_reducible_ex c k st); auto.
+    + destruct H3 as [_ [_ ?]].
+      apply WP_Pre; auto.
+      intros.
+      pose proof H3 _ _ _ _ H5 as (c1' & k1' & ? & ?).
+      
+
+      revert H H2 H5 H6.
+      clear.
+      intros.
+
+      remember (c, k, st) as prog.
+      remember (c1', k1', st') as prog'.
+      rewrite Heqprog in *. rewrite Heqprog' in *.
+      rewrite <- Heqprog in H5. rewrite <- Heqprog' in H5.
+      revert c k st Heqprog H2 H6.
+
+      unfold mstep in H5.
+      apply clos_trans_t1n_iff in H5.
+      induction H5; intros; subst; [pose proof H2 _ _ _ H0 _ _ H6; auto |].
+      destruct y as [[c'' k''] st''].
+      specialize (IHclos_trans_1n eq_refl _ _ _ eq_refl).
+
+
+      specialize (H2 _ _ _ H)
+    + destruct H3 as [_ [? _]].
+      apply H3 in H4.
+      exfalso; apply (reducible_irreducible_ex c k st); auto.
+
     apply WP_Pre.
     + apply H in H3.
       destruct H3 as [_ [? _]].
-      unfold Error in H3.
     
     apply Hsym in H3.
       specialize (H _ _ _ _ H3) as [_ ?].
@@ -69,7 +188,7 @@ Proof.
       specialize (H _ _ _ _ H3) as [_ ?].
       specialize (H _ _ _ _ H4) as (c2' & k2' & ? & ?).
       specialize (H2 _ _ _ H _ _ H5). auto.
-Admitted.
+Admitted. *)
 
 
 
